compiler/backend/languages/semantics/thunkLang_primitivesScript.sml
@@ -249,5 +249,13 @@ Proof
   \\ strip_tac \\ gvs []
 QED
 
+Datatype:
+  mop = Ret | Bind
+      | Raise | Handle
+      | Act
+      | Alloc | Length | Deref | Update
+End
+
+
 val _ = export_theory ();
 
